io/case-study/Shared.fst
@@ -1,8 +1,0 @@
-module Shared
-
-open FStar.Tactics
-open FStar.Classical.Sugar
-
-open Compiler.Model
-
-assume val shr : src_interface
